# 三角函数

澡尔冯的辣鸡三角函数

> 参考维基百科

## 导数

### 三角函数

$$
(\sin x)\prime=\cos x
$$

$$
(\cos x)\prime=-\sin x
$$

$$
(\tan x)\prime=\frac{1}{\cos^2 x}=\sec^2 x
$$

$$
(\cot x)\prime=-\frac{1}{\sin^2 x}=-\csc^2 x
$$

$$
(\sec x)\prime=\sec x\tan x
$$

$$
(\csc x)\prime=-\csc x\cot x
$$

### 反三角函数

$$
(\arcsin x)\prime=\frac{1}{\sqrt{1-x^2}} (\lvert x\rvert \lt 1)
$$

$$
(\arccos x)\prime=-\frac{1}{\sqrt{1-x^2}} (\lvert x\rvert \lt 1)
$$

$$
(\arctan x)\prime=\frac{1}{1+x^2}
$$

$$
(\operatorname{arccot} x)\prime=-\frac{1}{1+x^2}
$$

$$
(\operatorname{arcsec} x)\prime=\frac{1}{\lvert x \rvert\sqrt{x^2-1}} (\lvert x\rvert \gt 1)
$$

$$
(\operatorname{arccsc} x)\prime=-\frac{1}{\lvert x\rvert\sqrt{x^2-1}} (\lvert x\rvert \gt 1)
$$

## 积化和差

$$
\sin a\sin b=\frac{1}{2}(\cos (a-b)-\cos (a+b))
$$

$$
\cos a\cos b=\frac{1}{2}(\cos (a-b)+\cos (a+b))
$$

$$
\sin a\cos b=\frac{1}{2}(\sin (a+b)+\sin (a-b))
$$

$$
\cos a\sin b=\frac{1}{2}(\sin (a+b)-\sin (a-b))
$$

$$
\sin a+\sin b=2\sin\frac{a+b}{2}\cos\frac{a-b}{2}
$$

$$
\sin a-\sin b=2\cos\frac{a+b}{2}\sin\frac{a-b}{2}
$$

$$
\cos a+\cos b=2\cos\frac{a+b}{2}\cos\frac{a-b}{2}
$$

$$
\cos a-\cos b=-2\sin\frac{a+b}{2}\sin\frac{a-b}{2}
$$

$$
\tan a\tan b=\frac{\cos (a-b)-\cos (a+b)}{\cos (a-b)+\cos (a+b)}
$$

$$
\tan a\cot b=\frac{\sin (a+b)+\sin (a-b)}{\sin (a+b)-\sin (a-b)}
$$

## 和差公式

$$
\sin(\alpha\pm\beta)=\sin\alpha\cos\beta\pm\cos\alpha\sin\beta
$$

$$
\cos(\alpha\pm\beta)=\cos\alpha\cos\beta\mp\sin\alpha\sin\beta
$$

$$
\tan(\alpha\pm\beta)=\frac{\tan\alpha\pm\tan\beta}{1\mp\tan\alpha\tan\beta}
$$

$$
\cot(\alpha\pm\beta)=\frac{\cot\alpha\cot\beta\mp1}{\cot\beta\pm\cot\alpha}
$$

$$
\sec(\alpha\pm\beta)=\frac{\sec\alpha\sec\beta\csc\alpha\csc\beta}{\csc\alpha\csc\beta\mp\sec\alpha\sec\beta}
$$

$$
\csc(\alpha\pm\beta)=\frac{\sec\alpha\sec\beta\csc\alpha\csc\beta}{\sec\alpha\csc\beta\pm\csc\alpha\sec\beta}
$$

$$
\arcsin x\pm\arcsin y=\arcsin(x\sqrt{1-y^2}\pm y\sqrt{1-x^2})
$$

$$
\arccos x\pm\arccos y=\arccos(xy\mp\sqrt{(1-x^2)(1-y^2)})
$$

$$
\arctan x\pm\arctan y=\arctan\frac{x\pm y}{1\mp xy}
$$

$$
\operatorname{arccot}x\pm\operatorname{arccot}y=\operatorname{arccot}\frac{xy\mp 1}{y\pm x}
$$

## 倍角公式

### 二倍角

$$
{\displaystyle \sin(2\theta )=2\sin \theta \cos \theta =(\sin \theta +\cos \theta )^{2}-1={\frac {2\tan \theta }{1+\tan ^{2}\theta }}}
$$

$$
{\displaystyle \cos(2\theta )=\cos ^{2}\theta -\sin ^{2}\theta =2\cos ^{2}\theta -1=1-2\sin ^{2}\theta ={\frac {1-\tan ^{2}\theta }{1+\tan ^{2}\theta }}}
$$

$$
{\displaystyle \tan(2\theta )={\frac {2\tan \theta }{1-\tan ^{2}\theta }}}
$$

$$
{\displaystyle \cot(2\theta )={\frac {\cot ^{2}\theta -1}{2\cot \theta }}={\frac {1-\tan ^{2}\theta }{2\tan \theta }}}
$$

$$
{\displaystyle \sec(2\theta )={\frac {\sec ^{2}\theta }{2-\sec ^{2}\theta }}={\frac {1+\tan ^{2}\theta }{1-\tan ^{2}\theta }}}
$$

$$
{\displaystyle \csc(2\theta )={\frac {\sec \theta \csc \theta }{2}}={\frac {1+\tan ^{2}\theta }{2\tan \theta }}}
$$

### 三倍角

$$
{\displaystyle \sin(3\theta )=3\sin \theta -4\sin ^{3}\theta =4\sin \theta \sin \left({\frac {\pi }{3}}-\theta \right)\sin \left({\frac {\pi }{3}}+\theta \right)}
$$

$$
{\displaystyle \cos(3\theta )=4\cos ^{3}\theta -3\cos \theta =4\cos \theta \cos \left({\frac {\pi }{3}}-\theta \right)\cos \left({\frac {\pi }{3}}+\theta \right)}
$$

$$
{\displaystyle \tan(3\theta )={\frac {3\tan \theta -\tan ^{3}\theta }{1-3\tan ^{2}\theta }}=\tan \theta \tan \left({\frac {\pi }{3}}-\theta \right)\tan \left({\frac {\pi }{3}}+\theta \right)}
$$

$$
{\displaystyle \cot(3\theta )={\frac {3\cot \theta -\cot ^{3}\theta }{1-3\cot ^{2}\theta }}}
$$

$$
{\displaystyle \sec(3\theta )={\frac {\sec ^{3}\theta }{4-3\sec ^{2}\theta }}}
$$

$$
{\displaystyle \csc(3\theta )={\frac {\csc ^{3}\theta }{3\csc ^{2}\theta -4}}}
$$

## 半角公式

$$
{\displaystyle {\begin{aligned}\sin {\frac {\theta }{2}}&=\operatorname {sgn} \left(\sin {\frac {\theta }{2}}\right){\sqrt {\frac {1-\cos \theta }{2}}}\\[3pt]\cos {\frac {\theta }{2}}&=\operatorname {sgn} \left(\cos {\frac {\theta }{2}}\right){\sqrt {\frac {1+\cos \theta }{2}}}\\[3pt]\tan {\frac {\theta }{2}}&={\frac {1-\cos \theta }{\sin \theta }}={\frac {\sin \theta }{1+\cos \theta }}=\csc \theta -\cot \theta ={\frac {\tan \theta }{1+\sec {\theta }}}\\[6mu]&=\operatorname {sgn}(\sin \theta ){\sqrt {\frac {1-\cos \theta }{1+\cos \theta }}}={\frac {-1+\operatorname {sgn}(\cos \theta ){\sqrt {1+\tan ^{2}\theta }}}{\tan \theta }}\\[3pt]\cot {\frac {\theta }{2}}&={\frac {1+\cos \theta }{\sin \theta }}={\frac {\sin \theta }{1-\cos \theta }}=\csc \theta +\cot \theta =\operatorname {sgn}(\sin \theta ){\sqrt {\frac {1+\cos \theta }{1-\cos \theta }}}\\\sec {\frac {\theta }{2}}&=\operatorname {sgn} \left(\cos {\frac {\theta }{2}}\right){\sqrt {\frac {2}{1+\cos \theta }}}\\\csc {\frac {\theta }{2}}&=\operatorname {sgn} \left(\sin {\frac {\theta }{2}}\right){\sqrt {\frac {2}{1-\cos \theta }}}\\\end{aligned}}}
$$

## 降幂公式

| Sine                                                                                           | Cosine                                                                                         | Other                                                                                                              |
| ---------------------------------------------------------------------------------------------- | ---------------------------------------------------------------------------------------------- | ------------------------------------------------------------------------------------------------------------------ |
| ${\displaystyle \sin ^{2}\theta ={\frac {1-\cos(2\theta )}{2}}}$                               | ${\displaystyle \cos ^{2}\theta ={\frac {1+\cos(2\theta )}{2}}}$                               | ${\displaystyle \sin ^{2}\theta \cos ^{2}\theta ={\frac {1-\cos(4\theta )}{8}}}$                                   |
| ${\displaystyle \sin ^{3}\theta ={\frac {3\sin \theta -\sin(3\theta )}{4}}}$                   | ${\displaystyle \cos ^{3}\theta ={\frac {3\cos \theta +\cos(3\theta )}{4}}}$                   | ${\displaystyle \sin ^{3}\theta \cos ^{3}\theta ={\frac {3\sin(2\theta )-\sin(6\theta )}{32}}}$                    |
| ${\displaystyle \sin ^{4}\theta ={\frac {3-4\cos(2\theta )+\cos(4\theta )}{8}}}$               | ${\displaystyle \cos ^{4}\theta ={\frac {3+4\cos(2\theta )+\cos(4\theta )}{8}}}$               | ${\displaystyle \sin ^{4}\theta \cos ^{4}\theta ={\frac {3-4\cos(4\theta )+\cos(8\theta )}{128}}}$                 |
| ${\displaystyle \sin ^{5}\theta ={\frac {10\sin \theta -5\sin(3\theta )+\sin(5\theta )}{16}}}$ | ${\displaystyle \cos ^{5}\theta ={\frac {10\cos \theta +5\cos(3\theta )+\cos(5\theta )}{16}}}$ | ${\displaystyle \sin ^{5}\theta \cos ^{5}\theta ={\frac {10\sin(2\theta )-5\sin(6\theta )+\sin(10\theta )}{512}}}$ |

## 级数展开

$$
{\displaystyle \sin x=x-{\frac {x^{3}}{3!}}+{\frac {x^{5}}{5!}}-{\frac {x^{7}}{7!}}+\cdots =\sum _{n=0}^{\infty }{\frac {(-1)^{n}x^{2n+1}}{(2n+1)!}},}
$$

$$
{\displaystyle \cos x=1-{\frac {x^{2}}{2!}}+{\frac {x^{4}}{4!}}-{\frac {x^{6}}{6!}}+\cdots =\sum _{n=0}^{\infty }{\frac {(-1)^{n}x^{2n}}{(2n)!}}.}
$$

## 积分公式

$$
\int\tan xdx=-\ln\lvert\cos x\rvert+C
$$

$$
\int\cot xdx=-\ln\lvert\sin x\rvert+C
$$

$$
\int\sec xdx=\ln\lvert\sec x+\tan x\rvert+C
$$

$$
\int\csc xdx=\ln\lvert\csc x-\cot x\rvert+C
$$

$$
\int\frac{dx}{a^2+x^2}=\frac{1}{a}\arctan\frac{x}{a}+C
$$

$$
\int\frac{dx}{x^2-a^2}=\frac{1}{2a}\ln\left|\frac{x-a}{x+a}\right|+c
$$

$$
\int\frac{dx}{\sqrt{a^2-x^2}}=\arcsin\frac{x}{a}+C
$$

$$
\int\frac{dx}{\sqrt{x^2+a^2}}=\ln(x+\sqrt{x^2+a^2})+C
$$

$$
\int\frac{dx}{\sqrt{x^2-a^2}}=\ln(x+\sqrt{x^2-a^2})+C
$$

## 沃利斯乘积

$$
\int_0^{\frac{\pi}{2}}\sin^nxdx=\int_0^{\frac{\pi}{2}}\cos^nxdx=
\left\{
\begin{aligned}
    \frac{n-1}{n}\cdot\frac{n-3}{n-2}\ldots\frac{3}{4}\cdot\frac{1}{2}\cdot\frac{\pi}{2} \\
    \frac{n-1}{n}\cdot\frac{n-3}{n-2}\ldots\frac{6}{7}\cdot\frac{4}{5}\cdot\frac{2}{3}\cdot 1 \\
\end{aligned}
\right.
$$
